% YOUR SOLUTION TO PROBLEM 2 GOES HERE
% THE LATEX CODE YOU PUT HERE WILL BE INLINED (IF YOU NEED ADD ANY PACKAGES DO IT IN THE MAIN TEMPLATE FILE)

By using Observation 6 from the lecture notes we can deduce:

\begin{align*}
\forall x \in \Sigma^* s.t. \  \hat \delta (q_0,x) \in F: \hat \delta(q_0, x) \notin \overline F, thus \ x \in L(M) \rightarrow x \notin L(\overline M). \\
\forall y \in \Sigma^* s.t. \  \hat \delta (q_0, y) \notin  F: \hat \delta(q_0, y) \in \overline F, thus \ y \notin L(M) \rightarrow y \in L(\overline M). \\
\end{align*}
$$
\text{Therefore, } L(\overline M) = \Sigma^* - L(M) = \overline{L(M)}
$$